first version of Advanced Inductive Defs section

doc-src/TutorialI/Inductive/Advanced.thy
@@ -1,67 +1,222 @@
 (* ID:         $Id$ *)
 theory Advanced = Even:
 
-text{* We completely forgot about "rule inversion", or whatever we may want
-to call it. Just as a demo I include the two forms that Markus has made available. First the one for binding the result to a name *}
 
-inductive_cases even_cases [elim!]:
-  "Suc(Suc n) \<in> even"
+datatype 'f gterm = Apply 'f "'f gterm list"
 
-thm even_cases;
+datatype integer_op = Number int | UnaryMinus | Plus;
 
-text{*and now the one for local usage:*}
-
-lemma "Suc(Suc n) \<in> even \<Longrightarrow> n \<in> even";
-by(ind_cases "Suc(Suc n) \<in> even");
-
-text{*Both forms accept lists of strings.
-
-Hope you can find some more exciting examples, although these may do
-*}
-
-
-datatype 'f "term" = Apply 'f "'f term list"
-
-consts terms :: "'f set \<Rightarrow> 'f term set"
-inductive "terms F"
+consts gterms :: "'f set \<Rightarrow> 'f gterm set"
+inductive "gterms F"
 intros
-step[intro]: "\<lbrakk>\<forall>t \<in> set term_list. t \<in> terms F;  f \<in> F\<rbrakk>
-              \<Longrightarrow> (Apply f term_list) \<in> terms F"
+step[intro!]: "\<lbrakk>\<forall>t \<in> set args. t \<in> gterms F;  f \<in> F\<rbrakk>
+               \<Longrightarrow> (Apply f args) \<in> gterms F"
 
-
-lemma "F\<subseteq>G \<Longrightarrow> terms F \<subseteq> terms G"
+lemma gterms_mono: "F\<subseteq>G \<Longrightarrow> gterms F \<subseteq> gterms G"
 apply clarify
-apply (erule terms.induct)
+apply (erule gterms.induct)
 apply blast
 done
 
-consts term_type :: "('f \<Rightarrow> 't list * 't) \<Rightarrow> ('f term * 't)set"
-inductive "term_type sig"
-intros
-step[intro]: "\<lbrakk>\<forall>et \<in> set term_type_list. et \<in> term_type sig; 
-               sig f = (map snd term_type_list, rtype)\<rbrakk>
-              \<Longrightarrow> (Apply f (map fst term_type_list), rtype) \<in> term_type sig"
+text{*
+The situation after induction
 
-consts term_type' :: "('f \<Rightarrow> 't list * 't) \<Rightarrow> ('f term * 't)set"
-inductive "term_type' sig"
+proof\ {\isacharparenleft}prove{\isacharparenright}{\isacharcolon}\ step\ {\isadigit{2}}\isanewline
+\isanewline
+goal\ {\isacharparenleft}lemma{\isacharparenright}{\isacharcolon}\isanewline
+F\ {\isasymsubseteq}\ G\ {\isasymLongrightarrow}\ gterms\ F\ {\isasymsubseteq}\ gterms\ G\isanewline
+\ {\isadigit{1}}{\isachardot}\ {\isasymAnd}x\ args\ f{\isachardot}\isanewline
+\ \ \ \ \ \ \ {\isasymlbrakk}F\ {\isasymsubseteq}\ G{\isacharsemicolon}\ {\isasymforall}t{\isasymin}set\ args{\isachardot}\ t\ {\isasymin}\ gterms\ F\ {\isasymand}\ t\ {\isasymin}\ gterms\ G{\isacharsemicolon}\ f\ {\isasymin}\ F{\isasymrbrakk}\isanewline
+\ \ \ \ \ \ \ {\isasymLongrightarrow}\ Apply\ f\ args\ {\isasymin}\ gterms\ G
+*}
+
+text{* We completely forgot about "rule inversion". 
+
+@{thm[display] even.cases[no_vars]}
+\rulename{even.cases}
+
+Just as a demo I include
+the two forms that Markus has made available. First the one for binding the
+result to a name 
+
+*}
+
+inductive_cases Suc_Suc_cases [elim!]:
+  "Suc(Suc n) \<in> even"
+
+thm Suc_Suc_cases;
+
+text{*
+@{thm[display] Suc_Suc_cases[no_vars]}
+\rulename{Suc_Suc_cases}
+
+and now the one for local usage:
+*}
+
+lemma "Suc(Suc n) \<in> even \<Longrightarrow> P n";
+apply (ind_cases "Suc(Suc n) \<in> even");
+oops
+
+inductive_cases gterm_Apply_elim [elim!]: "Apply f args \<in> gterms F"
+
+text{*this is what we get:
+
+@{thm[display] gterm_Apply_elim[no_vars]}
+\rulename{gterm_Apply_elim}
+*}
+
+lemma gterms_IntI [rule_format]:
+     "t \<in> gterms F \<Longrightarrow> t \<in> gterms G \<longrightarrow> t \<in> gterms (F\<inter>G)"
+apply (erule gterms.induct)
+apply blast
+done
+
+
+text{*
+Subgoal after induction.  How would we cope without rule inversion?
+
+pr(latex xsymbols symbols)
+
+proof\ {\isacharparenleft}prove{\isacharparenright}{\isacharcolon}\ step\ {\isadigit{1}}\isanewline
+\isanewline
+goal\ {\isacharparenleft}lemma\ gterms{\isacharunderscore}IntI{\isacharparenright}{\isacharcolon}\isanewline
+t\ {\isasymin}\ gterms\ F\ {\isasymLongrightarrow}\ t\ {\isasymin}\ gterms\ G\ {\isasymlongrightarrow}\ t\ {\isasymin}\ gterms\ {\isacharparenleft}F\ {\isasyminter}\ G{\isacharparenright}\isanewline
+\ {\isadigit{1}}{\isachardot}\ {\isasymAnd}args\ f{\isachardot}\isanewline
+\ \ \ \ \ \ \ {\isasymlbrakk}{\isasymforall}t{\isasymin}set\ args{\isachardot}\ t\ {\isasymin}\ gterms\ F\ {\isasymand}\ {\isacharparenleft}t\ {\isasymin}\ gterms\ G\ {\isasymlongrightarrow}\ t\ {\isasymin}\ gterms\ {\isacharparenleft}F\ {\isasyminter}\ G{\isacharparenright}{\isacharparenright}{\isacharsemicolon}\isanewline
+\ \ \ \ \ \ \ \ \ \ f\ {\isasymin}\ F{\isasymrbrakk}\isanewline
+\ \ \ \ \ \ \ {\isasymLongrightarrow}\ Apply\ f\ args\ {\isasymin}\ gterms\ G\ {\isasymlongrightarrow}\ Apply\ f\ args\ {\isasymin}\ gterms\ {\isacharparenleft}F\ {\isasyminter}\ G{\isacharparenright}
+
+
+*}
+
+text{*
+@{thm[display] mono_Int[no_vars]}
+\rulename{mono_Int}
+*}
+
+lemma gterms_Int_eq [simp]:
+     "gterms (F\<inter>G) = gterms F \<inter> gterms G"
+apply (rule equalityI)
+apply (blast intro!: mono_Int monoI gterms_mono)
+apply (blast intro!: gterms_IntI)
+done
+
+
+consts integer_arity :: "integer_op \<Rightarrow> nat"
+primrec
+"integer_arity (Number n)        = #0"
+"integer_arity UnaryMinus        = #1"
+"integer_arity Plus              = #2"
+
+consts well_formed_gterm :: "('f \<Rightarrow> nat) \<Rightarrow> 'f gterm set"
+inductive "well_formed_gterm arity"
 intros
-step[intro]: "\<lbrakk>term_type_list \<in> lists(term_type' sig); 
-                 sig f = (map snd term_type_list, rtype)\<rbrakk>
-              \<Longrightarrow> (Apply f (map fst term_type_list), rtype) \<in> term_type' sig"
+step[intro!]: "\<lbrakk>\<forall>t \<in> set args. t \<in> well_formed_gterm arity;  
+                length args = arity f\<rbrakk>
+               \<Longrightarrow> (Apply f args) \<in> well_formed_gterm arity"
+
+
+consts well_formed_gterm' :: "('f \<Rightarrow> nat) \<Rightarrow> 'f gterm set"
+inductive "well_formed_gterm' arity"
+intros
+step[intro!]: "\<lbrakk>args \<in> lists (well_formed_gterm' arity);  
+                length args = arity f\<rbrakk>
+               \<Longrightarrow> (Apply f args) \<in> well_formed_gterm' arity"
+monos lists_mono
+
+lemma "well_formed_gterm arity \<subseteq> well_formed_gterm' arity"
+apply clarify
+apply (erule well_formed_gterm.induct)
+apply auto
+done
+
+
+text{*
+The situation after clarify (note the induction hypothesis!)
+
+pr(latex xsymbols symbols)
+
+proof\ {\isacharparenleft}prove{\isacharparenright}{\isacharcolon}\ step\ {\isadigit{2}}\isanewline
+\isanewline
+goal\ {\isacharparenleft}lemma{\isacharparenright}{\isacharcolon}\isanewline
+well{\isacharunderscore}formed{\isacharunderscore}gterm\ arity\ {\isasymsubseteq}\ well{\isacharunderscore}formed{\isacharunderscore}gterm{\isacharprime}\ arity\isanewline
+\ {\isadigit{1}}{\isachardot}\ {\isasymAnd}x\ args\ f{\isachardot}\isanewline
+\ \ \ \ \ \ \ {\isasymlbrakk}{\isasymforall}t{\isasymin}set\ args{\isachardot}\isanewline
+\ \ \ \ \ \ \ \ \ \ \ t\ {\isasymin}\ well{\isacharunderscore}formed{\isacharunderscore}gterm\ arity\ {\isasymand}\ t\ {\isasymin}\ well{\isacharunderscore}formed{\isacharunderscore}gterm{\isacharprime}\ arity{\isacharsemicolon}\isanewline
+\ \ \ \ \ \ \ \ \ \ length\ args\ {\isacharequal}\ arity\ f{\isasymrbrakk}\isanewline
+\ \ \ \ \ \ \ {\isasymLongrightarrow}\ Apply\ f\ args\ {\isasymin}\ well{\isacharunderscore}formed{\isacharunderscore}gterm{\isacharprime}\ arity
+*}
+
+
+lemma "well_formed_gterm' arity \<subseteq> well_formed_gterm arity"
+apply clarify
+apply (erule well_formed_gterm'.induct)
+apply auto
+done
+
+
+text{*
+@{thm[display] lists_Int_eq[no_vars]}
+\rulename{lists_Int_eq}
+
+The situation after clarify (note the strange induction hypothesis!)
+
+pr(latex xsymbols symbols)
+
+proof\ {\isacharparenleft}prove{\isacharparenright}{\isacharcolon}\ step\ {\isadigit{2}}\isanewline
+\isanewline
+goal\ {\isacharparenleft}lemma{\isacharparenright}{\isacharcolon}\isanewline
+well{\isacharunderscore}formed{\isacharunderscore}gterm{\isacharprime}\ arity\ {\isasymsubseteq}\ well{\isacharunderscore}formed{\isacharunderscore}gterm\ arity\isanewline
+\ {\isadigit{1}}{\isachardot}\ {\isasymAnd}x\ args\ f{\isachardot}\isanewline
+\ \ \ \ \ \ \ {\isasymlbrakk}args\isanewline
+\ \ \ \ \ \ \ \ {\isasymin}\ lists\isanewline
+\ \ \ \ \ \ \ \ \ \ \ {\isacharparenleft}well{\isacharunderscore}formed{\isacharunderscore}gterm{\isacharprime}\ arity\ {\isasyminter}\ {\isacharbraceleft}u{\isachardot}\ u\ {\isasymin}\ well{\isacharunderscore}formed{\isacharunderscore}gterm\ arity{\isacharbraceright}{\isacharparenright}{\isacharsemicolon}\isanewline
+\ \ \ \ \ \ \ \ \ \ length\ args\ {\isacharequal}\ arity\ f{\isasymrbrakk}\isanewline
+\ \ \ \ \ \ \ {\isasymLongrightarrow}\ Apply\ f\ args\ {\isasymin}\ well{\isacharunderscore}formed{\isacharunderscore}gterm\ arity
+*}
+
+text{* the rest isn't used: too complicated.  OK for an exercise though.*}
+
+consts integer_signature :: "(integer_op * (unit list * unit)) set"
+inductive "integer_signature"
+intros
+Number:     "(Number n,   ([], ())) \<in> integer_signature"
+UnaryMinus: "(UnaryMinus, ([()], ())) \<in> integer_signature"
+Plus:       "(Plus,       ([(),()], ())) \<in> integer_signature"
+
+
+consts well_typed_gterm :: "('f \<Rightarrow> 't list * 't) \<Rightarrow> ('f gterm * 't)set"
+inductive "well_typed_gterm sig"
+intros
+step[intro!]: 
+    "\<lbrakk>\<forall>pair \<in> set args. pair \<in> well_typed_gterm sig; 
+      sig f = (map snd args, rtype)\<rbrakk>
+     \<Longrightarrow> (Apply f (map fst args), rtype) 
+         \<in> well_typed_gterm sig"
+
+consts well_typed_gterm' :: "('f \<Rightarrow> 't list * 't) \<Rightarrow> ('f gterm * 't)set"
+inductive "well_typed_gterm' sig"
+intros
+step[intro!]: 
+    "\<lbrakk>args \<in> lists(well_typed_gterm' sig); 
+      sig f = (map snd args, rtype)\<rbrakk>
+     \<Longrightarrow> (Apply f (map fst args), rtype) 
+         \<in> well_typed_gterm' sig"
 monos lists_mono
 
 
-lemma "term_type sig \<subseteq> term_type' sig"
+lemma "well_typed_gterm sig \<subseteq> well_typed_gterm' sig"
 apply clarify
-apply (erule term_type.induct)
+apply (erule well_typed_gterm.induct)
 apply auto
 done
 
-lemma "term_type' sig \<subseteq> term_type sig"
+lemma "well_typed_gterm' sig \<subseteq> well_typed_gterm sig"
 apply clarify
-apply (erule term_type'.induct)
+apply (erule well_typed_gterm'.induct)
 apply auto
 done
+
 
 end
 
